Left hand side
<p>
$$\begin{aligned}\overline{\bigg(\frac{z}{z'}\bigg)} &=  \overline{\bigg(\frac{x+iy}{x'+iy'}\bigg)}\\
&= \overline{\bigg(\frac{(x+iy)(x'-iy')}{(x'+iy')(x'-iy')}\bigg)}\\
&= \overline{\bigg(\frac{(x+iy)(x'-iy')}{(x'^2+y'^2)}\bigg)}\\
&= \overline{\bigg(\frac{xx'+yy'+i(x'y-xy')}{(x'^2+y'^2)}\bigg)}\\
&= \frac{xx'+yy'-i(x'y-xy')}{(x'^2+y'^2)}\\
\end{aligned} $$

Right hand side
<p>



$$\begin{aligned}\frac{\overline{z}}{\enspace \overline{z'} \enspace} &= \frac{\overline{x+iy}}{\enspace \overline{x'+iy'} \enspace}\\
&= \frac{x-iy}{\enspace x'-iy' \enspace}\\
&= \frac{(x-iy)(x'+iy')}{\enspace (x'-iy')(x'+iy') \enspace}\\
&= \frac{xx'+yy'-i(x'y-xy')}{\enspace (x'^2+y'^2) \enspace}\\
\end{aligned}$$
