<p>
$$\begin{aligned}
2z +i\overline{z} &= 4\\
2(x+iy) + i(x-iy) &= 4\\
2x +2iy +ix +y &= 4\\
2x +y +i (x + 2y) &= 4\\
\end{aligned}$$
<p>
$$
\begin{cases}
2x +y = 4\\
x + 2y = 0
\end{cases}
$$
<p>
$$
\begin{cases}
2x +y = 4\\
x = - 2y 
\end{cases}
$$
<p>


$$ 2(-2y) + y = 4 $$
$$ -4y +y = 4 $$
$$ -3y = 4$$
$$ \boxed{y = \frac{-4}{3}}$$

<p>
$$ x = -2(\frac{-4}{3})$$
$$\boxed{ x = \frac{8}{3}} $$

<p>

Verification $ z = \frac{8}{3}-i\frac{4}{3} $ ?
$$\begin{aligned}
 2z +i\overline{z} &= 2\bigg(\frac{8}{3}-i\frac{4}{3}\bigg)  + i \bigg(\frac{8}{3}+i\frac{4}{3}\bigg) \\
 &= \frac{16}{3}-i\frac{8}{3}  + i\frac{8}{3}-\frac{4}{3} \\
 &= \frac{12}{3}\\
 &= 4

\end{aligned}$$

$$ \boxed{z = \frac{8}{3}-i\frac{4}{3}} $$
